Update Chapter3.

Chapter3.thy
@@ -49,4 +49,62 @@ fun asimp :: "aexp \<Rightarrow> aexp" where
 "asimp (V x) = V x" |
 "asimp (Plus a1 a2) = plus (asimp a1) (asimp a2)"
 
+datatype bexp = Bc bool | Not bexp | And bexp bexp | Less aexp aexp
+
+fun bval :: "bexp \<Rightarrow> state \<Rightarrow> bool" where
+"bval (Bc b) s = b"
+| "bval (Not b) s = (\<not> (bval b s))"
+| "bval (And b1 b2) s = ((bval b1 s) \<and> (bval b2 s))"
+| "bval (Less a1 a2) s = (aval a1 s < aval a2 s)"
+
+fun not :: "bexp \<Rightarrow> bexp" where
+"not (Bc True) = Bc False"
+| "not (Bc False) = Bc True"
+| "not b = Not b"
+
+fun "and" :: "bexp \<Rightarrow> bexp \<Rightarrow> bexp" where
+"and (Bc True) b = b"
+| "and b (Bc True) = b"
+| "and (Bc False) b = (Bc False)"
+| "and b (Bc False) = (Bc False)"
+| "and b1 b2 = And b1 b2"
+
+fun less :: "aexp \<Rightarrow> aexp \<Rightarrow> bexp" where
+"less (N n1) (N n2) = Bc (n1 < n2)"
+| "less a1 a2 = Less a1 a2"
+
+fun bsimp :: "bexp \<Rightarrow> bexp" where
+"bsimp (Bc b) = Bc b"
+| "bsimp (Not b) = Not (bsimp b)"
+| "bsimp (And b1 b2) = And (bsimp b1) (bsimp b2)"
+| "bsimp (Less a1 a2) = less (asimp a1) (asimp a2)"
+
+datatype instr = LOADI val | LOAD vname | ADD
+
+type_synonym stack = "val list"
+
+fun exec1 :: "instr \<Rightarrow> state \<Rightarrow> stack \<Rightarrow> stack" where
+"exec1 (LOADI v) s stk = (v # stk)"
+| "exec1 (LOAD name) s stk = (s name # stk)"
+| "exec1 ADD s (x#y#stk) = ((x+y)#stk) "
+
+fun exec :: "instr list \<Rightarrow> state \<Rightarrow> stack \<Rightarrow> stack" where
+"exec [] _ stk = stk"
+| "exec (i#is) s stk = exec is s (exec1 i s stk)"
+
+fun comp :: "aexp \<Rightarrow> instr list" where
+"comp (N n) = [LOADI n]"
+| "comp (V x) = [LOAD x]"
+| "comp (Plus e1 e2) = comp e1 @ comp e2 @ [ADD]"
+
+lemma [simp]: "exec (is1 @ is2) s stk = exec is2 s (exec is1 s stk)"
+  apply(induction is1 arbitrary: stk)
+   apply(auto)
+  done
+
+lemma "exec (comp a) s stk = aval a s # stk"
+  apply(induction a arbitrary: stk)
+    apply(auto)
+  done
+
 end
