Exercise3.thy
@@ -11,10 +11,10 @@ type_synonym val = int
 datatype aexp = N val | V vname | Plus aexp aexp
 type_synonym state = "vname \<Rightarrow> val"
 
-fun aval :: "aexp \<Rightarrow> state \<Rightarrow> int" where
-"aval (N n) s = n" |
-"aval (V v) s = s v" |
-"aval (Plus a1 a2) s = (aval a1 s) + (aval a2 s)"
+fun aval :: "aexp \<Rightarrow> state \<Rightarrow> val" where
+"aval (N a) s = a" |
+"aval (V x) s = s x" |
+"aval (Plus a b) s = aval a s + aval b s"
 
 fun asimp_const :: "aexp \<Rightarrow> aexp" where
 "asimp_const (V v) = V v" |
@@ -26,12 +26,24 @@ case (asimp_const a1, asimp_const a2) of
 (b1, b2) \<Rightarrow> Plus b1 b2
 )"
 
+fun plus :: "aexp \<Rightarrow> aexp \<Rightarrow> aexp" where
+"plus (N a) (N b) = N (a+b)" |
+"plus p (N i) = (if i = 0 then p else Plus p (N i))" |
+"plus (N i) p = (if i = 0 then p else Plus (N i) p)" |
+"plus p q = (Plus p q)"
+
+fun asimp :: "aexp \<Rightarrow> aexp" where
+"asimp (N a) = N a" |
+"asimp (V x) = V x" |
+"asimp (Plus p q) = plus (asimp p) (asimp q)"
+
+
 (* Exer 3.1 *)
 fun optimal :: "aexp \<Rightarrow> bool" where
 "optimal (V v) = True" |
 "optimal (N n) = True" |
 "optimal (Plus (N n1) (N n2)) = False" |
-"optimal (Plus a1 a2) = conj (optimal a1) (optimal a2)"
+"optimal (Plus a1 a2) = ((optimal a1) \<and> (optimal a2))"
 
 theorem "optimal (asimp_const x)"
   apply(induction x)
@@ -71,13 +83,14 @@ value "subst ''x'' (N 10) (V ''y'')"
 value "subst ''x'' (N 10) (V ''x'')"
 value "subst ''x'' (N 3) (Plus (V ''x'') (V ''y''))"
 
-theorem "aval (subst x a e) s = aval e (s(x := aval a s))"
+(* this theorem should be set simp for future proofs in 3.6 *)
+theorem [simp]: "aval (subst x a e) s = aval e (s(x := aval a s))"
   apply(induction e)
     apply(auto)
   done
 
 (* \<Longrightarrow> is a  \<Longrightarrow> *)
-theorem "aval a1 s = aval a2 s \<Longrightarrow> aval (subst x a1 e) s = aval (subst x a2 e) s"
+theorem [simp]: "aval a1 s = aval a2 s \<Longrightarrow> aval (subst x a1 e) s = aval (subst x a2 e) s"
   apply(induction e)
     apply(auto)
   done
@@ -116,14 +129,297 @@ theorem "aval2 (asimp2 a) s = aval2 a s"
 datatype aexp3 = N3 int | V3 vname | Plus3 aexp3 aexp3 | Times3 aexp3 aexp3 | Post3 vname | Div3 aexp3 aexp3
 
 fun aval3 :: "aexp3 \<Rightarrow> state \<Rightarrow> (val* state)" where
-"aval3 (N3 n) s = (n, s)" |
-"aval3 (V3 v) s = (s v, s)" |
-"aval3 (Plus3 a1 a2) s = (fst (aval3 a1 s) + fst (aval3 a2 s), (\<lambda> x. (snd (aval3 a1 s) x + snd (aval3 a2 s) x - s x)))" |
-"aval3 (Times3 a1 a2) s = (fst (aval3 a1 s) * fst (aval3 a2 s), (\<lambda> x. (snd (aval3 a1 s) x + snd (aval3 a2 s) x - s x)))" |
-"aval3 (Post3 v) s = (s v + 1, (s(v := s v + 1)))" |
-"aval3 (Div3 a1 a2) s = (fst (aval3 a1 s) div fst (aval3 a2 s), (\<lambda> x. (snd (aval3 a1 s) x + snd (aval3 a2 s) x - s x)))"
+"aval3 (N3 n) s = (n, s)"
+| "aval3 (V3 v) s = (s v, s)"
+| "aval3 (Post3 v) s = (s v, s(v := s v + 1))"
+| "aval3 (Plus3 a1 a2) s = (fst (aval3 a1 s) + fst (aval3 a2 (snd (aval3 a1 s))), snd (aval3 a2 (snd (aval3 a1 s))))"
+| "aval3 (Times3 a1 a2) s = (fst (aval3 a1 s) * fst (aval3 a2 (snd (aval3 a1 s))), snd (aval3 a2 (snd (aval3 a1 s))))"
+| "aval3 (Div3 a1 a2) s = (fst (aval3 a1 s) div fst (aval3 a2 (snd (aval3 a1 s))), snd (aval3 a2 (snd (aval3 a1 s))))"
 
 value "aval3 (Div3 (N3 9) (V3 y))  (\<lambda> x. 3) "
 value "aval3 (Post3 v)  (\<lambda> x. 12) "
+
+fun aval3_2 :: "aexp3 \<Rightarrow> state \<Rightarrow> (val * state) option" where
+"aval3_2 (N3 n) s = Some (n, s)"
+| "aval3_2 (V3 v) s = Some (s v, s)"
+| "aval3_2 (Post3 v) s = Some (s v, s(v := s v + 1))"
+| "aval3_2 (Plus3 a1 a2) s = (
+   case (aval3_2 a1 s) of
+   None \<Rightarrow> None
+   | Some (v1, s1) \<Rightarrow>
+     (case (aval3_2 a2 s1) of
+      None \<Rightarrow> None
+      | Some (v2, s2) \<Rightarrow> Some (v1 + v2, s2)))"
+| "aval3_2 (Times3 a1 a2) s = (
+   case (aval3_2 a1 s) of
+   None \<Rightarrow> None 
+   | Some (v1, s1) \<Rightarrow>
+     (case (aval3_2 a2 s1) of
+      None \<Rightarrow> None
+      | Some (v2, s2) \<Rightarrow> Some (v1*v2, s2)))"
+| "aval3_2 (Div3 a1 a2) s = (
+   case (aval3_2 a1 s) of
+   None \<Rightarrow> None
+   | Some (v1, s1) \<Rightarrow>
+     (case (aval3_2 a2 s1) of
+      None \<Rightarrow> None
+      | Some (v2, s2) \<Rightarrow> (if v2 = 0 then None else Some (v1 div v2, s2))))"
+
+value "aval3_2 (Plus3 (Post3 x) (Post3 x)) (\<lambda> x. 0)"
+value "aval3_2 (Div3 (Post3 x) (N3 1))  (\<lambda> x. 3) "
+value "aval3_2 (Div3 (N3 9) (V3 y))  (\<lambda> x. 3) "
+value "aval3_2 (Div3 (N3 9) (V3 y))  (\<lambda> x. 0) "
+value "aval3_2 (Post3 v)  (\<lambda> x. 12) "
+value "aval3_2 (Plus3 (Post3 v) (Post3 v))  (\<lambda> x. 12) "
+value "aval3_2 (Times3 (Post3 v) (Post3 v))  (\<lambda> x. 12) "
+value "aval3_2 (Times3 (N3 9) (Div3 (V3 t) (N3 0)))  (\<lambda> x. 10) "
+value "aval3_2 (Times3 (N3 9) (Div3 (Post3 t) (Post3 z)))  (\<lambda> x. 10) "
+value "aval3_2 (Times3 (Div3 (V3 z) (N3 0)) (Div3 (V3 t) (N3 0)))  (\<lambda> x. 10) "
+
+(* Exer 3.6 *)
+datatype lexp = Nl int | Vl vname | Plusl lexp lexp | LET vname lexp lexp
+
+fun lval :: "lexp \<Rightarrow> state \<Rightarrow> int" where
+"lval (Nl a) s = a" |
+"lval (Vl x) s = s x" |
+"lval (Plusl p q) s = lval p s + lval q s" |
+"lval (LET x a e) s = lval e (s(x:=lval a s))"
+
+fun inline :: "lexp \<Rightarrow> aexp" where
+"inline (Nl a) = (N a)" |
+"inline (Vl x) = (V x)" |
+"inline (Plusl p q) = Plus (inline p) (inline q)" |
+"inline (LET x a e) = subst x (inline a) (inline e)"  
+
+theorem "aval (inline e) s = lval e s"
+apply (induction e arbitrary: s)
+apply (auto)
+done
+
+
+(* Exer 3.7 *)
+datatype bexp = Bc bool | Not bexp | And bexp bexp | Less aexp aexp
+
+definition Le :: "aexp \<Rightarrow> aexp \<Rightarrow> bexp" where
+"Le a1 a2 = Not (Less a2 a1)"
+
+definition Eq :: "aexp \<Rightarrow> aexp \<Rightarrow> bexp" where
+"Eq a1 a2 = And (Not (Less a1 a2)) (Not (Less a2 a1))"
+
+fun bval :: "bexp \<Rightarrow> state \<Rightarrow> bool" where
+"bval (Bc b) s = b"
+| "bval (Not b) s = (\<not> (bval b s))"
+| "bval (And b1 b2) s = ((bval b1 s) \<and> (bval b2 s))"
+| "bval (Less a1 a2) s = (aval a1 s < aval a2 s)"
+
+fun not :: "bexp \<Rightarrow> bexp" where
+"not (Bc True) = Bc False"
+| "not (Bc False) = Bc True"
+| "not b = Not b"
+
+fun "and" :: "bexp \<Rightarrow> bexp \<Rightarrow> bexp" where
+"and (Bc True) b = b"
+| "and b (Bc True) = b"
+| "and (Bc False) b = (Bc False)"
+| "and b (Bc False) = (Bc False)"
+| "and b1 b2 = And b1 b2"
+
+fun less :: "aexp \<Rightarrow> aexp \<Rightarrow> bexp" where
+"less (N n1) (N n2) = Bc (n1 < n2)"
+| "less a1 a2 = Less a1 a2"
+
+fun bsimp :: "bexp \<Rightarrow> bexp" where
+"bsimp (Bc b) = Bc b"
+| "bsimp (Not b) = Not (bsimp b)"
+| "bsimp (And b1 b2) = And (bsimp b1) (bsimp b2)"
+| "bsimp (Less a1 a2) = less (asimp a1) (asimp a2)"
+
+lemma bval_Eq: "bval (Eq a1 a2) s = (aval a1 s = aval a2 s)"
+  apply (auto simp add: Eq_def)
+  done  
+
+lemma bval_Le: "bval (Le a1 a2) s = (aval a1 s \<le> aval a2 s)"
+  apply (auto simp add: Le_def)
+  done 
+
+(* Exer 3.8 *)
+datatype ifexp = Bc2 bool | If ifexp ifexp ifexp | Less2 aexp aexp
+
+fun ifval :: "ifexp \<Rightarrow> state \<Rightarrow> bool" where
+"ifval (Bc2 c) s = c"
+| "ifval (Less2 a1 a2) s = (aval a1 s < aval a2 s)"
+| "ifval (If if1 if2 if3) s = (if (ifval if1 s) then (ifval if2 s) else (ifval if3 s))"
+
+fun b2ifexp :: "bexp \<Rightarrow> ifexp" where
+"b2ifexp (Bc b) = Bc2 b"
+| "b2ifexp (Less a1 a2) = Less2 a1 a2"
+| "b2ifexp (Not b) = (If (b2ifexp b) (Bc2 False) (Bc2 True))"
+| "b2ifexp (And b1 b2) = If (b2ifexp b1) (b2ifexp b2) (Bc2 False)"
+
+fun if2bexp :: "ifexp \<Rightarrow> bexp" where
+"if2bexp (Bc2 c) = Bc c"
+| "if2bexp (Less2 a1 a2) = Less a1 a2"
+| "if2bexp (If if1 if2 if3) = Not (And (Not (And (if2bexp if1) (if2bexp if2))) (Not (And (Not (if2bexp if1)) (if2bexp if3))))"
+(* (a&b) \<or> (\<not>a&c) = \<not>(\<not>(a&b) \<and> \<not>(\<not>a&c)) *)
+
+theorem "bval b s = ifval (b2ifexp b) s"
+  apply(induction b)
+     apply(auto)
+  done
+
+theorem "bval (if2bexp f) s = ifval f s"
+  apply(induction f)
+     apply(auto)
+  done
+
+(* Exer 3.9 *)
+datatype pbexp = VAR vname | NOT pbexp | AND pbexp pbexp | OR pbexp pbexp
+
+fun pbval :: "pbexp \<Rightarrow> (vname \<Rightarrow> bool) \<Rightarrow> bool" where
+"pbval (VAR x) s = s x"  
+| "pbval (NOT b) s = (\<not> (pbval b s))"
+| "pbval (AND b1 b2) s = ((pbval b1 s) \<and> (pbval b2 s))" 
+| "pbval (OR b1 b2) s = ((pbval b1 s) \<or> (pbval b2 s))"
+
+fun is_nnf :: "pbexp \<Rightarrow> bool" where
+"is_nnf (VAR v) = True"
+| "is_nnf (NOT (VAR v)) = True"
+| "is_nnf (NOT p) = False"
+| "is_nnf (AND p1 p2) = ((is_nnf p1) \<and> (is_nnf p2))"
+| "is_nnf (OR p1 p2) = ((is_nnf p1) \<and> (is_nnf p2))"
+
+fun nnf :: "pbexp \<Rightarrow> pbexp" where
+"nnf (VAR v) = VAR v"
+| "nnf (NOT (VAR v)) = NOT (VAR v)"
+| "nnf (AND p1 p2) = AND (nnf p1) (nnf p2)"
+| "nnf (OR p1 p2) = OR (nnf p1) (nnf p2)"
+| "nnf (NOT (NOT p)) = nnf p"
+| "nnf (NOT (AND p1 p2)) = OR (nnf (NOT p1)) (nnf (NOT p2))"
+| "nnf (NOT (OR p1 p2)) = AND (nnf (NOT p1)) (nnf (NOT p2))"
+
+lemma [simp]: "pbval (nnf (NOT p)) s = (\<not> pbval (nnf p) s)"
+  apply(induction p)
+     apply(auto)
+  done
+
+theorem "pbval (nnf p) s = pbval p s"                                  
+  apply(induction p)
+     apply(auto)
+  done
+
+theorem "is_nnf (nnf p)"
+  apply(induction p rule: nnf.induct)
+     apply(auto)
+  done
+
+(* Exer 3.10 *)
+datatype instr = LOADI val | LOAD vname | ADD
+type_synonym stack = "val list"
+
+fun exec1_modi :: "instr \<Rightarrow> state \<Rightarrow> stack \<Rightarrow> stack option" where
+"exec1_modi (LOADI v) s stk = Some (v#stk)"
+| "exec1_modi (LOAD v) s stk = Some (s v # stk)"
+| "exec1_modi ADD s (x#y#stk) = Some ((x+y)#stk)"
+| "exec1_modi ADD s stk = None"
+
+fun exec_modi :: "instr list \<Rightarrow> state \<Rightarrow> stack \<Rightarrow> stack option" where
+"exec_modi [] s stk = Some stk"
+| "exec_modi (x#xs) s stk = (
+     case (exec1_modi x s stk) of
+        None \<Rightarrow> None
+        | Some stk2 \<Rightarrow> exec_modi xs s stk2)"
+
+fun comp :: "aexp \<Rightarrow> instr list" where
+"comp (N n) = [LOADI n]"
+| "comp (V x) = [LOAD x]"
+| "comp (Plus e1 e2) = comp e1 @ comp e2 @ [ADD]"
+
+lemma [simp]: "exec_modi s1 s stk = Some stk1 \<Longrightarrow> exec_modi (s1@s2) s stk = exec_modi s2 s stk1"
+  apply(induction s1 arbitrary: stk)
+   apply(auto split: option.split)
+  done
+
+theorem "exec_modi (comp a) s stk = Some ((aval a s) # stk)"
+  apply(induction a arbitrary: stk)
+    apply(auto)
+  done
+
+(* Exer 3.11 *)
+type_synonym reg = nat
+datatype instr2 = LDI int reg | LD vname reg | ADD reg reg
+
+fun exec1 :: "instr2 \<Rightarrow> state \<Rightarrow> (reg \<Rightarrow> int) \<Rightarrow> reg \<Rightarrow> int" where
+"exec1 (LDI n r) s1 s2 = s2(r := n)"
+| "exec1 (LD n r) s1 s2 = s2(r := s1 n)"
+| "exec1 (ADD r1 r2) s1 s2 = s2(r1 := s2 r1 + s2 r2)"
+
+fun exec :: "instr2 list \<Rightarrow> state \<Rightarrow> (reg \<Rightarrow> int) \<Rightarrow> reg \<Rightarrow> int" where
+"exec [] s1 s2 = s2"
+| "exec (x#xs) s1 s2 = exec xs s1 (exec1 x s1 s2)"
+
+fun compiler :: "aexp \<Rightarrow> reg \<Rightarrow> instr2 list" where
+"compiler (N n) r = [LDI n r]"
+| "compiler (V v) r = [LD v r]"
+| "compiler (Plus a1 a2) r = (compiler a1 r) @ (compiler a2 (r+1)) @ [ADD r (r+1)]"
+
+lemma [simp]: "exec (a@b) s1 s2 = exec b s1 (exec a s1 s2)"
+  apply(induction a arbitrary: s2)
+   apply(auto)
+  done
+
+
+(* Meaning: compiler a q only affects those larger or equal to q, because in compiler we only mention q and q+1.
+   Thus, we do not change the key_value pair for those less than q in rs.
+ *)
+lemma [simp]: "q > r \<Longrightarrow> exec (compiler a q) s rs r = rs r"
+  apply(induction a arbitrary: r rs q)
+    apply(auto)
+  done
+
+theorem "exec (compiler a r) s rs r = aval a s"
+  apply(induction a arbitrary: r rs)
+   apply(auto)
+  done
+
+(* Exer 3.12 *)
+datatype instr0 = LDI0 val | LD0 vname | MV0 reg | ADD0 reg
+
+fun exec1_0 :: "instr0 \<Rightarrow> state \<Rightarrow> (reg \<Rightarrow> val) \<Rightarrow> reg \<Rightarrow> val" where
+"exec1_0 (LDI0 v) s rs = rs(0 := v)"
+| "exec1_0 (LD0 v) s rs = rs(0 := s v)"
+| "exec1_0 (MV0 r) s rs = rs(r := rs 0)"
+| "exec1_0 (ADD0 r1) s rs = rs(0 := rs 0 + rs r1)"
+
+fun exec0 :: "instr0 list \<Rightarrow> state \<Rightarrow> (reg \<Rightarrow> val) \<Rightarrow> reg \<Rightarrow> val" where
+"exec0 [] s rs = rs "
+| "exec0 (x#xs) s rs = exec0 xs s (exec1_0 x s rs)"
+
+fun compiler0 :: "aexp \<Rightarrow> reg \<Rightarrow> instr0 list" where
+"compiler0 (N n) r = [LDI0 n]"
+| "compiler0 (V v) r = [LD0 v]"
+| "compiler0 (Plus a1 a2) r = (compiler0 a1 (r+1)) @ [MV0 (r+1)] @ (compiler0 a2 (r+2)) @ [ADD0 (r+1)]"
+(* Note that: r may be 0. 
+ In this case, first put result a1 into 0
+ Second do nothing.
+ Third put result a2 into 0. Then data in 0 will be overwritten.
+ *)
+
+lemma [simp]: "exec0 (a@b) s rs = exec0 b s (exec0 a s rs)"
+  apply(induction a arbitrary: s rs b)
+   apply(auto)
+  done
+
+(* Meaning: compiler a q only affects those larger or equal to q, because in compiler we only mention q and q+1.
+   Thus, we do not change the key_value pair for those less than q in rs unless r is 0.
+ *)
+lemma [simp]: "r > 0 \<Longrightarrow> q > r \<Longrightarrow> exec0 (compiler0 a q) s rs r = rs r"
+  apply(induction a arbitrary: q s rs r)
+    apply(auto)
+  done
+
+theorem "exec0 (compiler0 a r) s rs 0 = aval a s"
+  apply(induction a arbitrary: r s rs)
+    apply(auto)
+  done
 
 end
