test.thy
@@ -1,0 +1,26 @@
+theory test
+imports Main
+
+begin
+type_synonym val = int
+type_synonym vname = string
+type_synonym state = "vname \<Rightarrow> val"
+
+datatype aexp2 = N2 int | V2 vname | Plus2 aexp2 aexp2 | PostInc vname 
+                        |  Times2 aexp2 aexp2 | Div2 aexp2 aexp2 
+fun aval2 :: "aexp2 \<Rightarrow> state \<Rightarrow> (val \<times> state)" where
+  "aval2 (N2 a) s = (a,s)" |
+  "aval2 (V2 x) s = (s x,s)" |
+  "aval2 (Plus2 a b) s = (fst (aval2 a s) + fst (aval2 b s), (\<lambda> x. (snd (aval2 a s) x) 
+  + (snd (aval2 b s) x) - (s x)))" |
+  "aval2 (PostInc x) s = (s x, s(x:= 1 + s x))" |
+  "aval2 (Times2 a b) s = (fst (aval2 a s) * fst (aval2 b s),(\<lambda> x. (snd (aval2 a s) x) 
+  + (snd (aval2 b s) x) - (s x)))" |  
+  "aval2 (Div2 a b) s = (fst (aval2 a s) div fst (aval2 b s),(\<lambda> x. (snd (aval2 a s) x) 
+  + (snd (aval2 b s) x) - (s x)))"
+  
+value "aval2 (Plus2 (PostInc x) (PostInc x)) (\<lambda> x. 0)"
+value "aval2 (Div2 (N2 9) (N2 3))  (\<lambda> x. 0) "
+value "aval2 (PostInc u)  (\<lambda> x. 0) "
+
+end
